Source/Concurrency/LinearTypeChecker.cs
@@ -423,7 +423,7 @@ namespace Microsoft.Boogie
           return null;
         case "Lheap_Write":
           return ExtractRootFromAccessPathExpr(callCmd.Ins[0]);
-        case "Lheap_Add":
+        case "Lheap_Alloc":
           return ExtractRootFromAccessPathExpr(callCmd.Ins[0]);
         case "Lheap_Remove":
           return ExtractRootFromAccessPathExpr(callCmd.Ins[0]);
